theories/reg_addr.v
@@ -1,23 +1,24 @@
+From Coq Require Import ssreflect ZArith.
 From HypVeri Require Import machine monad.
-From stdpp Require Import  fin_maps list countable fin  vector.
+From stdpp Require Import fin_maps list countable fin vector.
 
 Ltac solveWordSize :=
-  pose proof word_size_at_least as G;
-  unfold word_size_lower_bound in G;
+  pose proof word_size;
+  unfold word_size;
   lia.
 
 Ltac solveRegCount :=
-  pose proof reg_count_at_least as G;
-  unfold reg_count_lower_bound in G;
+  pose proof reg_count;
+  unfold reg_count;
   lia.
 
-Program Definition W0 : word := (@nat_to_fin 0 word_size _).
+Program Definition W0 : Word := (finz.FinZ 0 _ _).
 Solve Obligations with solveWordSize.
 
-Program Definition W1 : word := (@nat_to_fin 1 word_size _).
+Program Definition W1 : Word := (finz.FinZ 1 _ _).
 Solve Obligations with solveWordSize.
 
-Program Definition W2 : word := (@nat_to_fin 2 word_size _).
+Program Definition W2 : Word := (finz.FinZ 2 _ _).
 Solve Obligations with solveWordSize.
 
 Program Definition R0 :reg_name := (R 0 _).
@@ -28,35 +29,3 @@ Solve Obligations with solveRegCount.
 
 Program Definition R2 :reg_name := (R 2 _).
 Solve Obligations with solveRegCount.
-
-
-Definition incr_word (n : word) (p : nat) : option word :=
-  match (nat_lt_dec (n + p) word_size) with
-  | left l => Some (@nat_to_fin (n + p) _ l)
-  | _ => None
-  end.
-
-Infix "+w" := incr_word (at level 70, no associativity).
-
-Definition incr_word_unsafe (n : word) (p : nat) :  word :=
-  match (n +w p) with
-    | Some w => w
-    | None => W0
-  end.
-
-Infix "^+w" := incr_word_unsafe (at level 70, no associativity).
-
-
-(* Program Definition page_offset_to_addr (p :pid) (offset:fin page_size) : addr := *)
-(*   ((mm_translation_inv p)  !!! offset). *)
-
-(* Program Definition word_add (w:word) (n:nat):word:= *)
-(*   (@nat_to_fin (((fin_to_nat w)+n) mod word_size) _ _). *)
-(* Next Obligation. *)
-(* Proof. *)
-(*   intros. *)
-(*   apply mod_bound_pos. *)
-(*   lia. *)
-(*   pose proof word_size_at_least. *)
-(*   lia. *)
-(* Defined. *)
